Primitives for computing TInv and TMulN

cryptis/primitives/comp.v
@@ -16,6 +16,12 @@ Set Implicit Arguments.
 Unset Strict Implicit.
 Unset Printing Implicit Defensive.
 
+Definition tmul : val := λ: "t1" "t2", hl_mul "t1" "t2".
+
+Definition tinv : val := λ: "t", hl_inv_distr "t".
+
+Definition tone : val := λ: <>, hl_mk_mul NILV.
+
 Section Proofs.
 
 Context `{!heapGS Σ}.
@@ -77,5 +83,57 @@ Proof.
     rewrite -!val_of_pre_term_unfold (unfold_TInv_Nmul Nm).
     by iApply wp_hl_inv.
 Qed.
+
+Lemma twp_tmul E t1 t2 Ψ :
+  Ψ (TMulN [:: t1; t2]) ⊢
+  WP tmul t1 t2 @ E [{ Ψ }].
+Proof.
+iIntros "HΨ". rewrite /tmul; wp_lam; wp_pures.
+rewrite -[val_of_term t1]val_of_pre_term_unfold.
+rewrite -[val_of_term t2]val_of_pre_term_unfold.
+wp_apply twp_hl_mul.
+rewrite -(unfold_TMulN [:: t1; t2]) [repr _]val_of_pre_term_unfold.
+by iApply "HΨ".
+Qed.
+
+Lemma wp_tmul E t1 t2 Ψ :
+  Ψ (TMulN [:: t1; t2]) ⊢
+  WP tmul t1 t2 @ E {{ Ψ }}.
+Proof. by iIntros "post"; iApply twp_wp; iApply twp_tmul. Qed.
+
+Lemma twp_tinv E t Ψ :
+  Ψ (TInv t) ⊢
+  WP tinv t @ E [{ Ψ }].
+Proof.
+iIntros "HΨ". rewrite /tinv; wp_lam; wp_pures.
+rewrite -[val_of_term t]val_of_pre_term_unfold.
+wp_apply (twp_hl_inv_distr _ _ (wf_unfold_term t)).
+rewrite -unfold_TInv [repr _]val_of_pre_term_unfold.
+by iApply "HΨ".
+Qed.
+
+Lemma wp_tinv E t Ψ :
+  Ψ (TInv t) ⊢
+  WP tinv t @ E {{ Ψ }}.
+Proof. by iIntros "post"; iApply twp_wp; iApply twp_tinv. Qed.
+
+Lemma twp_tone E Ψ :
+  Ψ (TMulN [::]) ⊢
+  WP tone #() @ E [{ Ψ }].
+Proof.
+iIntros "HΨ". rewrite /tone; wp_pures.
+rewrite (_ : NILV = repr ([::] : seq PreTerm.pre_term));
+  last by rewrite repr_list_unseal.
+wp_apply (twp_hl_mk_mul E [::]).
+rewrite (_ : PreTerm.PTMul [::] = unfold_term (TMulN [::]));
+  last by rewrite (unfold_TMulN [::]).
+rewrite [repr _]val_of_pre_term_unfold.
+by iApply "HΨ".
+Qed.
+
+Lemma wp_tone E Ψ :
+  Ψ (TMulN [::]) ⊢
+  WP tone #() @ E {{ Ψ }}.
+Proof. by iIntros "post"; iApply twp_wp; iApply twp_tone. Qed.
 
 End Proofs.
